Mica/FOL/Variables.lean
@@ -8,6 +8,7 @@ import Mica.TinyML.RuntimeExpr
 inductive Srt where
   | int
   | bool
+  | bv (width : Nat)
   | char
   | string
   | float
@@ -19,6 +20,7 @@ inductive Srt where
 @[reducible] def Srt.denote : Srt → Type
   | .int => Int
   | .bool => Bool
+  | .bv width => BitVec width
   | .char => UInt8
   | .string => List UInt8
   | .float => UInt64
